add functions for parsing and serializing public keys

code/k256/Hacl.Impl.K256.Point.fst
@@ -16,6 +16,7 @@ module BI = Hacl.Spec.K256.Field52
 module BL = Hacl.Spec.K256.Field52.Lemmas
 
 open Hacl.K256.Field
+open Hacl.Impl.K256.Finv
 
 #set-options "--z3rlimit 50 --fuel 0 --ifuel 0"
 
@@ -108,39 +109,70 @@ let to_proj_point p x y =
 ///  Is a point in affine coordinates on the curve
 
 inline_for_extraction noextract
+val compute_expected_y2 (y2 x:felem) : Stack unit
+  (requires fun h ->
+    live h x /\ live h y2 /\ disjoint x y2 /\
+    inv_fully_reduced h x)
+  (ensures  fun h0 _ h1 -> modifies (loc y2) h0 h1 /\
+   (let xn = as_nat h0 x in inv_fully_reduced h1 y2 /\
+   as_nat h1 y2 == S.fadd (S.fmul (S.fmul xn xn) xn) S.b))
+
+let compute_expected_y2 y2 x =
+  push_frame ();
+  let b = create_felem () in
+
+  fsqr y2 x;
+  fmul y2 y2 x;
+  make_u52_5 b (make_b_k256 ());
+  let h0 = ST.get () in
+  assert (inv_lazy_reduced2 h0 y2);
+  assert (inv_fully_reduced h0 b);
+
+  BL.fadd5_lemma (1,1,1,1,2) (1,1,1,1,1) (as_felem5 h0 y2) (as_felem5 h0 b);
+  fadd y2 y2 b;
+  let h1 = ST.get () in
+  assert (felem_fits5 (as_felem5 h1 y2) (2,2,2,2,3));
+
+  fnormalize y2 y2;
+  BL.normalize5_lemma (2,2,2,2,3) (as_felem5 h1 y2);
+  pop_frame ()
+
+
+inline_for_extraction noextract
+val is_y_sqr_is_y2 (y2 y:felem) : Stack bool
+  (requires fun h ->
+    live h y /\ live h y2 /\ disjoint y y2 /\
+    inv_fully_reduced h y2 /\ inv_fully_reduced h y)
+  (ensures fun h0 b h1 -> modifies0 h0 h1 /\
+    b == (as_nat h0 y2 = S.fmul (as_nat h0 y) (as_nat h0 y)))
+
+let is_y_sqr_is_y2 y2 y =
+  push_frame ();
+  let y2_comp = create_felem () in
+
+  fsqr y2_comp y;
+  let h0 = ST.get () in
+  assert (inv_lazy_reduced2 h0 y2);
+  fnormalize y2_comp y2_comp;
+  BL.normalize5_lemma (1,1,1,1,2) (as_felem5 h0 y2_comp);
+
+  let res = is_felem_eq_vartime y2 y2_comp in
+  pop_frame ();
+  res
+
+
+inline_for_extraction noextract
 val is_on_curve_vartime (x y:felem) : Stack bool
   (requires fun h -> live h x /\ live h y /\
     inv_fully_reduced h x /\ inv_fully_reduced h y)
   (ensures  fun h0 b h1 -> modifies0 h0 h1 /\
-    b == S.is_on_curve (feval h0 x, feval h0 y))
+    b == S.is_on_curve (as_nat h0 x, as_nat h0 y))
 
 let is_on_curve_vartime x y =
   push_frame ();
-  let y2 = create_felem () in
-  let x3 = create_felem () in
-  let b = create_felem () in
-
-  let h = ST.get () in
-  fsqr y2 y;
-  fsqr x3 x;
-  fmul x3 x3 x;
-  make_u52_5 b (make_b_k256 ());
-  let h0 = ST.get () in
-  assert (inv_lazy_reduced2 h0 y2);
-  assert (inv_lazy_reduced2 h0 x3);
-  assert (inv_fully_reduced h0 b);
-
-  BL.fadd5_lemma (1,1,1,1,2) (1,1,1,1,1) (as_felem5 h0 x3) (as_felem5 h0 b);
-  fadd x3 x3 b;
-  let h1 = ST.get () in
-  assert (felem_fits5 (as_felem5 h1 x3) (2,2,2,2,3));
-
-  fnormalize x3 x3;
-  fnormalize y2 y2;
-  BL.normalize5_lemma (2,2,2,2,3) (as_felem5 h1 x3);
-  BL.normalize5_lemma (1,1,1,1,2) (as_felem5 h0 y2);
-
-  let res = is_felem_eq_vartime y2 x3 in
+  let y2_exp = create_felem () in
+  compute_expected_y2 y2_exp x;
+  let res = is_y_sqr_is_y2 y2_exp y in
   pop_frame ();
   res
 
@@ -161,5 +193,62 @@ let is_proj_point_at_inf_vartime p =
   BL.normalize5_lemma (1,1,1,1,2) (as_felem5 h0 pz);
   fnormalize tmp pz;
   let b = is_felem_zero_vartime tmp in
+  pop_frame ();
+  b
+
+
+inline_for_extraction noextract
+val recover_y_vartime (y x:felem) (is_odd:bool) : Stack bool
+  (requires fun h ->
+    live h x /\ live h y /\ disjoint x y /\
+    inv_fully_reduced h x /\ 0 < as_nat h x)
+  (ensures fun h0 b h1 -> modifies (loc y) h0 h1 /\
+    (b <==> Some? (S.recover_y (as_nat h0 x) is_odd)) /\
+    (b ==> (inv_fully_reduced h1 y /\
+      as_nat h1 y == Some?.v (S.recover_y (as_nat h0 x) is_odd))))
+
+let recover_y_vartime y x is_odd =
+  push_frame ();
+  let y2 = create_felem () in
+  compute_expected_y2 y2 x; //y2 = x *% x *% x +% b
+  fsqrt y y2;
+  let h = ST.get () in
+  BL.normalize5_lemma (1,1,1,1,2) (as_felem5 h y);
+  fnormalize y y;
+
+  let is_y_valid = is_y_sqr_is_y2 y2 y in
+  let res =
+    if not is_y_valid then false
+    else begin
+      let is_y_odd = is_fodd_vartime y in
+      fnegate_conditional_vartime y (is_y_odd <> is_odd);
+      true end in
+  pop_frame ();
+  res
+
+
+val recover_y_bytes_vartime (y x:lbuffer uint8 32ul) (is_odd:bool) : Stack bool
+  (requires fun h ->
+    live h x /\ live h y /\ disjoint x y)
+  (ensures fun h0 b h1 -> modifies (loc y) h0 h1 /\
+    (b <==> Some? (S.recover_y_bytes (as_seq h0 x) is_odd)) /\
+    (b ==> (as_seq h1 y == Some?.v (S.recover_y_bytes (as_seq h0 x) is_odd))))
+
+[@CInline]
+let recover_y_bytes_vartime y x is_odd =
+  push_frame ();
+  let xf = create_felem () in
+  let yf = create_felem () in
+  let is_x_valid = load_felem_vartime xf x in
+
+  let b =
+    if not is_x_valid then false
+    else begin
+      let r = recover_y_vartime yf xf is_odd in
+      if not r then false
+      else begin
+        store_felem y yf;
+        true end
+    end in
   pop_frame ();
   b
