code/k256/Hacl.K256.ECDSA.fst
@@ -12,22 +12,22 @@ module LSeq = Lib.Sequence
 module BSeq = Lib.ByteSequence
 
 module S = Spec.K256
+module BDL = Hacl.Spec.K256.Field52.Definitions.Lemmas
+
+module P = Hacl.Impl.K256.Point
 module SK = Hacl.Impl.K256.Sign
 module VK = Hacl.Impl.K256.Verify
 
 #set-options "--z3rlimit 50 --fuel 0 --ifuel 0"
 
-[@CInline]
 let ecdsa_sign_hashed_msg r s m private_key k =
   SK.ecdsa_sign_hashed_msg r s m private_key k
 
 
-[@CInline]
-let ecdsa_verify_hashed_msg m public_key_x public_key_y r s =
-  VK.ecdsa_verify_hashed_msg m public_key_x public_key_y r s
+let ecdsa_verify_hashed_msg m public_key r s =
+  VK.ecdsa_verify_hashed_msg m public_key r s
 
 
-[@CInline]
 let ecdsa_sign_sha256 r s msg_len msg private_key k =
   push_frame ();
   let mHash = create 32ul (u8 0) in
@@ -37,11 +37,74 @@ let ecdsa_sign_sha256 r s msg_len msg private_key k =
   b
 
 
-[@CInline]
-let ecdsa_verify_sha256 msg_len msg public_key_x public_key_y r s =
+let ecdsa_verify_sha256 msg_len msg public_key r s =
   push_frame ();
   let mHash = create 32ul (u8 0) in
   Hacl.Hash.SHA2.hash_256 msg msg_len mHash;
-  let b = ecdsa_verify_hashed_msg mHash public_key_x public_key_y r s in
+  let b = ecdsa_verify_hashed_msg mHash public_key r s in
   pop_frame ();
   b
+
+
+///  Parsing and Serializing public keys
+
+let pk_uncompressed_to_raw pk pk_raw =
+  let pk0 = pk.(0ul) in
+  if Lib.RawIntTypes.u8_to_UInt8 pk0 <> 0x04uy then false
+  else begin
+    copy pk_raw (sub pk 1ul 64ul);
+    true end
+
+
+let pk_uncompressed_from_raw pk_raw pk =
+  let h0 = ST.get () in
+  pk.(0ul) <- u8 0x04;
+  update_sub pk 1ul 64ul pk_raw;
+  let h1 = ST.get () in
+  LSeq.eq_intro (as_seq h1 pk) (S.pk_uncompressed_from_raw (as_seq h0 pk_raw))
+
+
+let pk_compressed_to_raw pk pk_raw =
+  let pk0 = pk.(0ul) in
+  if not (Lib.RawIntTypes.u8_to_UInt8 pk0 = 0x02uy ||
+    Lib.RawIntTypes.u8_to_UInt8 pk0 = 0x03uy) then false
+  else begin
+    let pk_xb = sub pk 1ul 32ul in
+    let is_pk_y_odd = Lib.RawIntTypes.u8_to_UInt8 pk0 = 0x03uy in
+    let pk_yb = sub pk_raw 32ul 32ul in
+    let b = P.recover_y_bytes_vartime pk_yb pk_xb is_pk_y_odd in
+    let h0 = ST.get () in
+    update_sub pk_raw 0ul 32ul pk_xb;
+    let h1 = ST.get () in
+    LSeq.eq_intro (as_seq h1 pk_raw) (LSeq.concat (as_seq h0 pk_xb) (as_seq h0 pk_yb));
+    b end
+
+
+inline_for_extraction noextract
+val is_nat_from_bytes_be_odd_vartime: f:lbytes 32ul -> Stack bool
+  (requires fun h -> live h f)
+  (ensures  fun h0 b h1 -> modifies0 h0 h1 /\
+    b == (BSeq.nat_from_bytes_be (as_seq h0 f) % 2 = 1))
+
+let is_nat_from_bytes_be_odd_vartime f =
+  let h0 = ST.get () in
+  let x0 = f.(31ul) in
+  BDL.lemma_nat_from_bytes_be_mod2 (as_seq h0 f);
+  [@inline_let]
+  let is_odd_m = x0 &. u8 1 in
+  mod_mask_lemma x0 1ul;
+  assert (v (mod_mask #U8 #SEC 1ul) == v (u8 1));
+  assert_norm (pow2 1 = 2);
+  assert (v is_odd_m = BSeq.nat_from_bytes_be (as_seq h0 f) % 2);
+  Lib.RawIntTypes.u8_to_UInt8 is_odd_m =. 1uy
+
+
+let pk_compressed_from_raw pk_raw pk =
+  let h0 = ST.get () in
+  let pk_x = sub pk_raw 0ul 32ul in
+  let pk_y = sub pk_raw 32ul 32ul in
+  let is_pk_y_odd = is_nat_from_bytes_be_odd_vartime pk_y in
+  pk.(0ul) <- if is_pk_y_odd then u8 0x03 else u8 0x02;
+  update_sub pk 1ul 32ul pk_x;
+  let h1 = ST.get () in
+  LSeq.eq_intro (as_seq h1 pk) (S.pk_compressed_from_raw (as_seq h0 pk_raw))
