code/k256/Hacl.K256.ECDSA.fsti
@@ -17,9 +17,9 @@ module S = Spec.K256
 #set-options "--z3rlimit 50 --fuel 0 --ifuel 0"
 
 inline_for_extraction noextract
-let lbytes32 = lbuffer uint8 32ul
+let lbytes len = lbuffer uint8 len
 
-val ecdsa_sign_hashed_msg (r s m private_key k:lbytes32) : Stack bool
+val ecdsa_sign_hashed_msg (r s m private_key k:lbytes 32ul) : Stack bool
   (requires fun h ->
     live h m /\ live h private_key /\ live h k /\
     live h r /\ live h s /\ disjoint r s /\
@@ -33,16 +33,15 @@ val ecdsa_sign_hashed_msg (r s m private_key k:lbytes32) : Stack bool
      as_seq h1 r == r_s /\ as_seq h1 s == s_s /\ b == b_s))
 
 
-val ecdsa_verify_hashed_msg (m public_key_x public_key_y r s:lbytes32) : Stack bool
+val ecdsa_verify_hashed_msg (m:lbytes 32ul) (public_key:lbytes 64ul) (r s:lbytes 32ul) : Stack bool
   (requires fun h ->
-    live h m /\ live h public_key_x /\ live h public_key_y /\
-    live h r /\ live h s /\ disjoint r s)
+    live h m /\ live h public_key /\ live h r /\
+    live h s /\ disjoint r s)
   (ensures fun h0 b h1 -> modifies0 h0 h1 /\
-    b == S.ecdsa_verify_hashed_msg (as_seq h0 m)
-      (as_seq h0 public_key_x) (as_seq h0 public_key_y) (as_seq h0 r) (as_seq h0 s))
+    b == S.ecdsa_verify_hashed_msg (as_seq h0 m) (as_seq h0 public_key) (as_seq h0 r) (as_seq h0 s))
 
 
-val ecdsa_sign_sha256 (r s:lbytes32) (msg_len:size_t) (msg:lbuffer uint8 msg_len) (private_key k:lbytes32) : Stack bool
+val ecdsa_sign_sha256 (r s:lbytes 32ul) (msg_len:size_t) (msg:lbytes msg_len) (private_key k:lbytes 32ul) : Stack bool
   (requires fun h ->
     live h msg /\ live h private_key /\ live h k /\
     live h r /\ live h s /\ disjoint r s /\
@@ -56,10 +55,37 @@ val ecdsa_sign_sha256 (r s:lbytes32) (msg_len:size_t) (msg:lbuffer uint8 msg_len
      as_seq h1 r == r_s /\ as_seq h1 s == s_s /\ b == b_s))
 
 
-val ecdsa_verify_sha256 (msg_len:size_t) (msg:lbuffer uint8 msg_len) (public_key_x public_key_y r s:lbytes32) : Stack bool
+val ecdsa_verify_sha256 (msg_len:size_t) (msg:lbytes msg_len) (public_key:lbytes 64ul) (r s:lbytes 32ul) : Stack bool
   (requires fun h ->
-    live h msg /\ live h public_key_x /\ live h public_key_y /\
-    live h r /\ live h s /\ disjoint r s)
+    live h msg /\ live h public_key /\ live h r /\
+    live h s /\ disjoint r s)
   (ensures fun h0 b h1 -> modifies0 h0 h1 /\
-    b == S.ecdsa_verify_sha256 (v msg_len) (as_seq h0 msg)
-      (as_seq h0 public_key_x) (as_seq h0 public_key_y) (as_seq h0 r) (as_seq h0 s))
+    b == S.ecdsa_verify_sha256 (v msg_len) (as_seq h0 msg) (as_seq h0 public_key) (as_seq h0 r) (as_seq h0 s))
+
+
+///  Parsing and Serializing public keys
+
+val pk_uncompressed_to_raw: pk:lbytes 65ul -> pk_raw:lbytes 64ul -> Stack bool
+  (requires fun h -> live h pk /\ live h pk_raw /\ disjoint pk pk_raw)
+  (ensures  fun h0 b h1 -> modifies (loc pk_raw) h0 h1 /\
+    (b <==> Some? (S.pk_uncompressed_to_raw (as_seq h0 pk))) /\
+    (b ==> (as_seq h1 pk_raw == Some?.v (S.pk_uncompressed_to_raw (as_seq h0 pk)))))
+
+
+val pk_uncompressed_from_raw: pk_raw:lbytes 64ul -> pk:lbytes 65ul -> Stack unit
+  (requires fun h -> live h pk /\ live h pk_raw /\ disjoint pk pk_raw)
+  (ensures  fun h0 _ h1 -> modifies (loc pk) h0 h1 /\
+    as_seq h1 pk == S.pk_uncompressed_from_raw (as_seq h0 pk_raw))
+
+
+val pk_compressed_to_raw: pk:lbytes 33ul -> pk_raw:lbytes 64ul -> Stack bool
+  (requires fun h -> live h pk /\ live h pk_raw /\ disjoint pk pk_raw)
+  (ensures  fun h0 b h1 -> modifies (loc pk_raw) h0 h1 /\
+    (b <==> Some? (S.pk_compressed_to_raw (as_seq h0 pk))) /\
+    (b ==> (as_seq h1 pk_raw == Some?.v (S.pk_compressed_to_raw (as_seq h0 pk)))))
+
+
+val pk_compressed_from_raw: pk_raw:lbytes 64ul -> pk:lbytes 33ul -> Stack unit
+  (requires fun h -> live h pk /\ live h pk_raw /\ disjoint pk pk_raw)
+  (ensures  fun h0 _ h1 -> modifies (loc pk) h0 h1 /\
+    as_seq h1 pk == S.pk_compressed_from_raw (as_seq h0 pk_raw))
